
#### basic equaiton
$  
\nabla\cdot{\bf{v}}=0   
$  
$
-\nabla P+\eta\nabla^2{\bf{v}}+\rho g \hat{e}_z=0
$  
$
\rho C(\frac{\partial T}{\partial t}+{\bf{v}} \cdot\nabla T)=k\nabla^2T+\rho H
$  
#### 无量纲
$x^,_i=x_i/D$  
$t^,=t\kappa/D^2$ because of $\sqrt{\kappa t_0}=D, t_0=D^2/\kappa$  
$v^,=vD/x$ because of $v_0=D/t_0 and v^,=v/v_0$  
$\rho=\rho_0-\rho_0\alpha(T-T_0)$ and $\rho_0,T_0$ are surface value    
P can be devided to two term:  
$P=p+\rho gz$  
dynamic pressure + hydrostatic pressure  

#### driviation
equation2:  
$-\nabla p-\rho g
\hat{e}_z+\eta\nabla^2{\bf{v}}+\rho g\hat{e}_z-\rho g\alpha(T-T_0) \hat{e}_z=0$  
then:  
$-\nabla p + \eta \nabla^2 {\bf{v}} - \rho_0 g \alpha(T-T_0) \hat{e}_z=0$  
---

$T^,=\frac{T-T_0}{T_b-T_0}$  
$p^,=\frac{pD^2}{\eta_0\kappa}$ because of $p=\eta/t=\frac{\eta_0\kappa}{D^2},  \eta:Pa\cdot s$  
$\eta^,=\eta/\eta_0$  
---
equation1:  
$\nabla {\bf{v}}=0$  
then:  
$\frac{\partial v}{\partial x}=\frac{\partial v_0v^,}{\partial x^,_i D}=\frac{v_0\partial v^,}{D\partial x^,_i}=\frac{\kappa\partial v^,}{D^2\partial x^,_i}$   
therefor:   
$\nabla{\bf{v^,}}=0$  

then:  
$- \frac{\eta_0\kappa}{D^3}\nabla p^,+\eta_0\eta^, \frac{\kappa}{D^2}\nabla^2{\bf{v^,}}+\rho_0 g \alpha(T_b-T_0)T^, \hat{e}_z=0$   
$-\nabla p^, + \eta^, \nabla^2 {\bf{v^,}}- \frac{\rho_0 g \alpha(T_b-T_0)D^3}{\eta_0 \kappa}T^, \hat{e}_z=0$  
where $\frac{\rho_0 g \alpha (T_b-T_0)D^3}{\eta_0\kappa}=Ra$   

equation3:  $\kappa=\frac{k}{\rho C}$
$\rho C[\frac{\partial (T-T_0)}{\partial t} + {\bf{v}}\nabla(T-T_0)]=k\nabla^2(T-T_0)+\rho H$  
$\rho C[\frac{\kappa \partial T^,}{D^2\partial  t^,}+\frac{\kappa}{D^2}{\bf{v}}\nabla T^,]=\frac{k}{D^2}\nabla^2 T^, + \frac{\rho H}{T_b-T_0}$   
$\frac{k}{D^2}[\frac{\partial T^,}{\partial t^,}+ {\bf{v^,}}\nabla T^,]=\frac{k}{D^2}\nabla^2 T^, +\frac{\rho H D^2}{(T_b-T_0)k}$   
$\frac{\partial T^,}{\partial t^,}+{\bf{v^,}}\nabla T^,=\nabla^2 T^, + \frac{\rho H D^2}{(T_b-T_0)k}$ where $\frac{\rho H D^2}{(T_b-T_0)k}=\gamma$   

#### the end
$\nabla{\bf{v^,}}=0$  
$-\nabla p^, + \eta^, \nabla^2 {\bf{v^,}}- R_a T^, \hat{e}_z=0$   
$\frac{\partial T^,}{\partial t^,}+{\bf{v^,}}\nabla T^,=\nabla^2 T^, + \gamma$